stdpp/gmap.v
@@ -1,139 +1,505 @@
-(** This file implements finite maps and finite sets with keys of any countable
-type. The implementation is based on [Pmap]s, radix-2 search trees.
+(** This files implements an efficient implementation of finite maps whose keys
+range over Coq's data type of any countable type [K]. The data structure is
+similar to [Pmap], which in turn is based on the "canonical" binary tries
+representation by Appel and Leroy, https://hal.inria.fr/hal-03372247. It thus
+has the same good properties:
 
-Computations on [gmap] or [gset], even concrete ones, are prevented from
-reducing with [simpl] or [cbv] (by marking [gmap_empty] as [Opaque]), because
-[simpl] reduces too eagerly.
-To compute concrete results, you need to both:
-- project in the end to some concrete data structure that, unlike
-  [gmap]/[gset], does not contain proofs, say via [map_to_list] or [!!]; and
-- use [vm_compute] to run the computation, because it ignores opacity.
-*)
+- It guarantees logarithmic-time [lookup] and [partial_alter], and linear-time
+  [merge]. It has a low constant factor for computation in Coq compared to other
+  versions (see the Appel and Leroy paper for benchmarks).
+- It satisfies extensional equality [(∀ i, m1 !! i = m2 !! i) → m1 = m2].
+- It can be used in nested recursive definitions, e.g.,
+  [Inductive test := Test : gmap test → test]. This is possible because we do
+  _not_ use a Sigma type to ensure canonical representations (a Sigma type would
+  break Coq's strict positivity check).
+
+Compared to [Pmap], we not only need to make sure the trie representation is
+canonical, we also need to make sure that all positions (of type positive) are
+valid encodings of [K]. That is, for each position [q] in the trie, we have:
+
+  encode <$> decode q = Some q
+
+Instead of formalizing this condition using a Sigma type (which would break
+the strict positivity check in nested recursive definitions), we make
+[gmap_dep_ne A P] dependent on a predicate [P : positive → Prop] that describes
+the subset of valid positions, and instantiate it with [gmap_key K].
+
+The predicate [P : positive → Prop] is considered irrelevant by extraction, so
+after extraction, the resulting data structure is identical to [Pmap]. *)
 From stdpp Require Export countable infinite fin_maps fin_map_dom.
-From stdpp Require Import pmap mapset propset.
+From stdpp Require Import mapset pmap.
 From stdpp Require Import options.
 
-(* FIXME: This file needs a 'Proof Using' hint, but they need to be set
-locally (or things moved out of sections) as no default works well enough. *)
-Unset Default Proof Using.
+Local Open Scope positive_scope.
 
-(** * The data structure *)
-(** We pack a [Pmap] together with a proof that ensures that all keys correspond
-to codes of actual elements of the countable type. *)
-Definition gmap_wf K `{Countable K} {A} (m : Pmap A) : Prop :=
-  bool_decide (map_Forall (λ p _, encode (A:=K) <$> decode p = Some p) m).
-Record gmap K `{Countable K} A := GMap {
-  gmap_car : Pmap A;
-  gmap_prf : gmap_wf K gmap_car
-}.
-Global Arguments GMap {_ _ _ _} _ _ : assert.
-Global Arguments gmap_car {_ _ _ _} _ : assert.
-Lemma gmap_eq `{Countable K} {A} (m1 m2 : gmap K A) :
-  m1 = m2 ↔ gmap_car m1 = gmap_car m2.
+Local Notation "P ~ 0" := (λ p, P p~0) : function_scope.
+Local Notation "P ~ 1" := (λ p, P p~1) : function_scope.
+Implicit Type P : positive → Prop.
+
+(** * The tree data structure *)
+Inductive gmap_dep_ne (A : Type) (P : positive → Prop) :=
+  | GNode001 : gmap_dep_ne A P~1  → gmap_dep_ne A P 
+  | GNode010 : P 1 → A → gmap_dep_ne A P
+  | GNode011 : P 1 → A → gmap_dep_ne A P~1 → gmap_dep_ne A P
+  | GNode100 : gmap_dep_ne A P~0 → gmap_dep_ne A P
+  | GNode101 : gmap_dep_ne A P~0 → gmap_dep_ne A P~1 → gmap_dep_ne A P
+  | GNode110 : gmap_dep_ne A P~0 → P 1 → A → gmap_dep_ne A P
+  | GNode111 : gmap_dep_ne A P~0 → P 1 → A → gmap_dep_ne A P~1 → gmap_dep_ne A P.
+Global Arguments GNode001 {A P} _ : assert.
+Global Arguments GNode010 {A P} _ _ : assert.
+Global Arguments GNode011 {A P} _ _ _ : assert.
+Global Arguments GNode100 {A P} _ : assert.
+Global Arguments GNode101 {A P} _ _ : assert.
+Global Arguments GNode110 {A P} _ _ _ : assert.
+Global Arguments GNode111 {A P} _ _ _ _ : assert.
+
+(** Using [Variant] we supress the generation of the induction scheme. We use
+the induction scheme [gmap_ind] in terms of the smart constructors to reduce the
+number of cases, similar to Appel and Leroy. *)
+Variant gmap_dep (A : Type) (P : positive → Prop) :=
+  | GEmpty : gmap_dep A P
+  | GNodes : gmap_dep_ne A P → gmap_dep A P.
+Global Arguments GEmpty {A P}.
+Global Arguments GNodes {A P} _.
+
+Record gmap_key K `{Countable K} (q : positive) :=
+  GMapKey { _ : encode (A:=K) <$> decode q = Some q }.
+Global Arguments GMapKey {_ _ _ _} _.
+
+Lemma gmap_key_encode `{Countable K} (k : K) : gmap_key K (encode k).
+Proof. constructor. by rewrite decode_encode. Qed.
+Global Instance gmap_key_pi `{Countable K} q : ProofIrrel (gmap_key K q).
+Proof. intros [?] [?]. f_equal. apply (proof_irrel _). Qed.
+
+Record gmap K `{Countable K} A := GMap { gmap_car : gmap_dep A (gmap_key K) }.
+Global Arguments GMap {_ _ _ _} _.
+Global Arguments gmap_car {_ _ _ _} _.
+
+Global Instance gmap_dep_ne_eq_dec {A P} :
+  EqDecision A → (∀ i, ProofIrrel (P i)) → EqDecision (gmap_dep_ne A P).
 Proof.
-  split; [by intros ->|intros]. destruct m1, m2; simplify_eq/=.
-  f_equal; apply proof_irrel.
-Qed.
-Global Instance gmap_eq_eq `{Countable K, EqDecision A} : EqDecision (gmap K A).
-Proof.
- refine (λ m1 m2, cast_if (decide (gmap_car m1 = gmap_car m2)));
-  abstract (by rewrite gmap_eq).
+  intros ? Hirr t1 t2. revert P t1 t2 Hirr.
+  refine (fix go {P} (t1 t2 : gmap_dep_ne A P) {Hirr : _} : Decision (t1 = t2) :=
+    match t1, t2 with
+    | GNode001 r1, GNode001 r2 => cast_if (go r1 r2)
+    | GNode010 _ x1, GNode010 _ x2 => cast_if (decide (x1 = x2))
+    | GNode011 _ x1 r1, GNode011 _ x2 r2 =>
+       cast_if_and (decide (x1 = x2)) (go r1 r2)
+    | GNode100 l1, GNode100 l2 => cast_if (go l1 l2)
+    | GNode101 l1 r1, GNode101 l2 r2 => cast_if_and (go l1 l2) (go r1 r2)
+    | GNode110 l1 _ x1, GNode110 l2 _ x2 =>
+       cast_if_and (go l1 l2) (decide (x1 = x2))
+    | GNode111 l1 _ x1 r1, GNode111 l2 _ x2 r2 =>
+       cast_if_and3 (go l1 l2) (decide (x1 = x2)) (go r1 r2)
+    | _, _ => right _
+    end);
+    clear go; abstract first [congruence|f_equal; done || apply Hirr|idtac].
 Defined.
+Global Instance gmap_dep_eq_dec {A P} :
+  (∀ i, ProofIrrel (P i)) → EqDecision A → EqDecision (gmap_dep A P).
+Proof. intros. solve_decision. Defined.
+Global Instance gmap_eq_dec `{Countable K} {A} :
+  EqDecision A → EqDecision (gmap K A).
+Proof. intros. solve_decision. Defined.
 
-(** * Operations on the data structure *)
-Global Instance gmap_lookup `{Countable K} {A} : Lookup K A (gmap K A) :=
-  λ i '(GMap m _), m !! encode i.
-Global Instance gmap_empty `{Countable K} {A} : Empty (gmap K A) := GMap ∅ I.
+(** The smart constructor [GNode] and eliminator [gmap_dep_ne_case] are used to
+reduce the number of cases, similar to Appel and Leroy. *)
+Local Definition GNode {A P}
+    (ml : gmap_dep A P~0)
+    (mx : option (P 1 * A)) (mr : gmap_dep A P~1) : gmap_dep A P :=
+  match ml, mx, mr with
+  | GEmpty, None, GEmpty => GEmpty
+  | GEmpty, None, GNodes r => GNodes (GNode001 r)
+  | GEmpty, Some (p,x), GEmpty => GNodes (GNode010 p x)
+  | GEmpty, Some (p,x), GNodes r => GNodes (GNode011 p x r)
+  | GNodes l, None, GEmpty => GNodes (GNode100 l)
+  | GNodes l, None, GNodes r => GNodes (GNode101 l r)
+  | GNodes l, Some (p,x), GEmpty => GNodes (GNode110 l p x)
+  | GNodes l, Some (p,x), GNodes r => GNodes (GNode111 l p x r)
+  end.
+
+Local Definition gmap_dep_ne_case {A P B} (t : gmap_dep_ne A P)
+    (f : gmap_dep A P~0 → option (P 1 * A) → gmap_dep A P~1 → B) : B :=
+  match t with
+  | GNode001 r => f GEmpty None (GNodes r)
+  | GNode010 p x => f GEmpty (Some (p,x)) GEmpty
+  | GNode011 p x r => f GEmpty (Some (p,x)) (GNodes r)
+  | GNode100 l => f (GNodes l) None GEmpty
+  | GNode101 l r => f (GNodes l) None (GNodes r)
+  | GNode110 l p x => f (GNodes l) (Some (p,x)) GEmpty
+  | GNode111 l p x r => f (GNodes l) (Some (p,x)) (GNodes r)
+  end.
+
+(** Operations *)
+Local Definition gmap_dep_ne_lookup {A} : ∀ {P}, positive → gmap_dep_ne A P → option A :=
+  fix go {P} i t {struct t} :=
+  match t, i with
+  | (GNode010 _ x | GNode011 _ x _ | GNode110 _ _ x | GNode111 _ _ x _), 1 => Some x
+  | (GNode100 l | GNode110 l _ _ | GNode101 l _ | GNode111 l _ _ _), i~0 => go i l
+  | (GNode001 r | GNode011 _ _ r | GNode101 _ r | GNode111 _ _ _ r), i~1 => go i r
+  | _, _ => None
+  end.
+Local Definition gmap_dep_lookup {A P}
+    (i : positive) (mt : gmap_dep A P) : option A :=
+  match mt with GEmpty => None | GNodes t => gmap_dep_ne_lookup i t end.
+Global Instance gmap_lookup `{Countable K} {A} :
+    Lookup K A (gmap K A) := λ k mt,
+  gmap_dep_lookup (encode k) (gmap_car mt).
+
+Global Instance gmap_empty `{Countable K} {A} : Empty (gmap K A) := GMap GEmpty.
+
 (** Block reduction, even on concrete [gmap]s.
 Marking [gmap_empty] as [simpl never] would not be enough, because of
 https://github.com/coq/coq/issues/2972 and
 https://github.com/coq/coq/issues/2986.
 And marking [gmap] consumers as [simpl never] does not work either, see:
-https://gitlab.mpi-sws.org/iris/stdpp/-/merge_requests/171#note_53216
-*)
+https://gitlab.mpi-sws.org/iris/stdpp/-/merge_requests/171#note_53216 *)
 Global Opaque gmap_empty.
 
-Lemma gmap_partial_alter_wf `{Countable K} {A} (f : option A → option A) m i :
-  gmap_wf K m → gmap_wf K (partial_alter f (encode (A:=K) i) m).
-Proof.
-  unfold gmap_wf; rewrite !bool_decide_spec.
-  intros Hm p x. destruct (decide (encode i = p)) as [<-|?].
-  - rewrite decode_encode; eauto.
-  - rewrite lookup_partial_alter_ne by done. by apply Hm.
-Qed.
+Local Fixpoint gmap_dep_ne_singleton {A P} (i : positive) :
+    P i → A → gmap_dep_ne A P :=
+  match i with
+  | 1 => GNode010
+  | i~0 => λ p x, GNode100 (gmap_dep_ne_singleton i p x)
+  | i~1 => λ p x, GNode001 (gmap_dep_ne_singleton i p x)
+  end.
+
+Local Definition gmap_partial_alter_aux {A P}
+    (go : ∀ i, P i → gmap_dep_ne A P → gmap_dep A P)
+    (f : option A → option A) (i : positive) (p : P i)
+    (mt : gmap_dep A P) : gmap_dep A P :=
+  match mt with
+  | GEmpty =>
+     match f None with
+     | None => GEmpty | Some x => GNodes (gmap_dep_ne_singleton i p x)
+     end
+  | GNodes t => go i p t
+  end.
+Local Definition gmap_dep_ne_partial_alter {A} (f : option A → option A) :
+    ∀ {P} (i : positive), P i → gmap_dep_ne A P → gmap_dep A P :=
+  Eval lazy -[gmap_dep_ne_singleton] in
+  fix go {P} i p t {struct t} :=
+    gmap_dep_ne_case t $ λ ml mx mr,
+      match i with
+      | 1 => λ p, GNode ml ((p,.) <$> f (snd <$> mx)) mr
+      | i~0 => λ p, GNode (gmap_partial_alter_aux go f i p ml) mx mr
+      | i~1 => λ p, GNode ml mx (gmap_partial_alter_aux go f i p mr)
+      end p.
+Local Definition gmap_dep_partial_alter {A P}
+    (f : option A → option A) : ∀ i : positive, P i → gmap_dep A P → gmap_dep A P :=
+  gmap_partial_alter_aux (gmap_dep_ne_partial_alter f) f.
 Global Instance gmap_partial_alter `{Countable K} {A} :
-    PartialAlter K A (gmap K A) := λ f i '(GMap m Hm),
-  GMap (partial_alter f (encode i) m) (gmap_partial_alter_wf f m i Hm).
+    PartialAlter K A (gmap K A) := λ f k '(GMap mt),
+  GMap $ gmap_dep_partial_alter f (encode k) (gmap_key_encode k) mt.
 
-Lemma gmap_fmap_wf `{Countable K} {A B} (f : A → B) m :
-  gmap_wf K m → gmap_wf K (f <$> m).
-Proof.
-  unfold gmap_wf; rewrite !bool_decide_spec.
-  intros ? p x. rewrite lookup_fmap, fmap_Some; intros (?&?&?); eauto.
-Qed.
-Global Instance gmap_fmap `{Countable K} : FMap (gmap K) := λ A B f '(GMap m Hm),
-  GMap (f <$> m) (gmap_fmap_wf f m Hm).
+Local Definition gmap_dep_ne_fmap {A B} (f : A → B) :
+    ∀ {P}, gmap_dep_ne A P → gmap_dep_ne B P :=
+  fix go {P} t :=
+    match t with
+    | GNode001 r => GNode001 (go r)
+    | GNode010 p x => GNode010 p (f x)
+    | GNode011 p x r => GNode011 p (f x) (go r)
+    | GNode100 l => GNode100 (go l)
+    | GNode101 l r => GNode101 (go l) (go r)
+    | GNode110 l p x => GNode110 (go l) p (f x)
+    | GNode111 l p x r => GNode111 (go l) p (f x) (go r)
+    end.
+Local Definition gmap_dep_fmap {A B P} (f : A → B)
+    (mt : gmap_dep A P) : gmap_dep B P :=
+  match mt with GEmpty => GEmpty | GNodes t => GNodes (gmap_dep_ne_fmap f t) end.
+Global Instance gmap_fmap `{Countable K} : FMap (gmap K) := λ {A B} f '(GMap mt),
+  GMap $ gmap_dep_fmap f mt.
 
-Lemma gmap_omap_wf `{Countable K} {A B} (f : A → option B) m :
-  gmap_wf K m → gmap_wf K (omap f m).
-Proof.
-  unfold gmap_wf; rewrite !bool_decide_spec.
-  intros ? p x; rewrite lookup_omap, bind_Some; intros (?&?&?); eauto.
-Qed.
-Global Instance gmap_omap `{Countable K} : OMap (gmap K) := λ A B f '(GMap m Hm),
-  GMap (omap f m) (gmap_omap_wf f m Hm).
+Local Definition gmap_dep_omap_aux {A B P}
+    (go : gmap_dep_ne A P → gmap_dep B P) (tm : gmap_dep A P) : gmap_dep B P :=
+  match tm with GEmpty => GEmpty | GNodes t' => go t' end.
+Local Definition gmap_dep_ne_omap {A B} (f : A → option B) :
+    ∀ {P}, gmap_dep_ne A P → gmap_dep B P :=
+  fix go {P} t :=
+    gmap_dep_ne_case t $ λ ml mx mr,
+      GNode (gmap_dep_omap_aux go ml) ('(p,x) ← mx; (p,.) <$> f x)
+            (gmap_dep_omap_aux go mr).
+Local Definition gmap_dep_omap {A B P} (f : A → option B) :
+  gmap_dep A P → gmap_dep B P := gmap_dep_omap_aux (gmap_dep_ne_omap f).
+Global Instance gmap_omap `{Countable K} : OMap (gmap K) := λ {A B} f '(GMap mt),
+  GMap $ gmap_dep_omap f mt.
 
-Lemma gmap_merge_wf `{Countable K} {A B C}
-    (f : option A → option B → option C) m1 m2 :
-  gmap_wf K m1 → gmap_wf K m2 → gmap_wf K (merge f m1 m2).
-Proof.
-  unfold gmap_wf; rewrite !bool_decide_spec.
-  intros Hm1 Hm2 p z. rewrite lookup_merge; intros.
-  destruct (m1 !! _) eqn:?, (m2 !! _) eqn:?; naive_solver.
-Qed.
+Local Definition gmap_merge_aux {A B C P}
+    (go : gmap_dep_ne A P → gmap_dep_ne B P → gmap_dep C P)
+    (f : option A → option B → option C)
+    (mt1 : gmap_dep A P) (mt2 : gmap_dep B P) : gmap_dep C P :=
+  match mt1, mt2 with
+  | GEmpty, GEmpty => GEmpty
+  | GNodes t1', GEmpty => gmap_dep_ne_omap (λ x, f (Some x) None) t1'
+  | GEmpty, GNodes t2' => gmap_dep_ne_omap (λ x, f None (Some x)) t2'
+  | GNodes t1', GNodes t2' => go t1' t2'
+  end.
+
+Local Definition diag_None' {A B C} {P : Prop}
+    (f : option A → option B → option C)
+    (mx : option (P * A)) (my : option (P * B)) : option (P * C) :=
+  match mx, my with
+  | None, None => None
+  | Some (p,x), None => (p,.) <$> f (Some x) None
+  | None, Some (p,y) => (p,.) <$> f None (Some y)
+  | Some (p,x), Some (_,y) => (p,.) <$> f (Some x) (Some y)
+  end.
+
+Local Definition gmap_dep_ne_merge {A B C} (f : option A → option B → option C) :
+    ∀ {P}, gmap_dep_ne A P → gmap_dep_ne B P → gmap_dep C P :=
+  fix go {P} t1 t2 {struct t1} :=
+    gmap_dep_ne_case t1 $ λ ml1 mx1 mr1,
+      gmap_dep_ne_case t2 $ λ ml2 mx2 mr2,
+        GNode (gmap_merge_aux go f ml1 ml2) (diag_None' f mx1 mx2)
+              (gmap_merge_aux go f mr1 mr2).
+Local Definition gmap_dep_merge {A B C P} (f : option A → option B → option C) :
+    gmap_dep A P → gmap_dep B P → gmap_dep C P :=
+  gmap_merge_aux (gmap_dep_ne_merge f) f.
 Global Instance gmap_merge `{Countable K} : Merge (gmap K) :=
-  λ A B C f '(GMap m1 Hm1) '(GMap m2 Hm2),
-    GMap (merge f m1 m2) (gmap_merge_wf f m1 m2 Hm1 Hm2).
+  λ {A B C} f '(GMap mt1) '(GMap mt2), GMap $ gmap_dep_merge f mt1 mt2.
 
-Global Instance gmap_fold `{Countable K} {A} : MapFold K A (gmap K A) :=
-  λ B f d '(GMap m _),
-    map_fold (λ i x, match decode i with Some k => f k x | None => id end) d m.
+Local Definition gmap_fold_aux {A B P}
+    (go : positive → B → gmap_dep_ne A P → B)
+    (i : positive) (y : B) (mt : gmap_dep A P) : B :=
+  match mt with GEmpty => y | GNodes t => go i y t end.
+Local Definition gmap_dep_ne_fold {A B} (f : positive → A → B → B) :
+    ∀ {P}, positive → B → gmap_dep_ne A P → B :=
+  fix go {P} i y t :=
+    gmap_dep_ne_case t $ λ ml mx mr,
+      gmap_fold_aux go i~1
+        (gmap_fold_aux go i~0
+          match mx with None => y | Some (p,x) => f (Pos.reverse i) x y end ml) mr.
+Local Definition gmap_dep_fold {A B P} (f : positive → A → B → B) :
+    positive → B → gmap_dep A P → B :=
+  gmap_fold_aux (gmap_dep_ne_fold f).
+Global Instance gmap_fold `{Countable K} {A} :
+    MapFold K A (gmap K A) := λ {B} f y '(GMap mt),
+  gmap_dep_fold (λ i x, match decode i with Some k => f k x | None => id end) 1 y mt.
 
-(** * Instantiation of the finite map interface *)
+(** Proofs *)
+Local Definition GNode_valid {A P}
+    (ml : gmap_dep A P~0) (mx : option (P 1 * A)) (mr : gmap_dep A P~1) :=
+  match ml, mx, mr with GEmpty, None, GEmpty => False | _, _, _ => True end.
+Local Lemma gmap_dep_ind A (Q : ∀ P, gmap_dep A P → Prop) :
+  (∀ P, Q P GEmpty) →
+  (∀ P ml mx mr, GNode_valid ml mx mr → Q _ ml → Q _ mr → Q P (GNode ml mx mr)) →
+  ∀ P mt, Q P mt.
+Proof.
+  intros Hemp Hnode P [|t]; [done|]. induction t.
+  - by apply (Hnode _ GEmpty None (GNodes _)).
+  - by apply (Hnode _ GEmpty (Some (_,_)) GEmpty).
+  - by apply (Hnode _ GEmpty (Some (_,_)) (GNodes _)).
+  - by apply (Hnode _ (GNodes _) None GEmpty).
+  - by apply (Hnode _ (GNodes _) None (GNodes _)).
+  - by apply (Hnode _ (GNodes _) (Some (_,_)) GEmpty).
+  - by apply (Hnode _ (GNodes _) (Some (_,_)) (GNodes _)).
+Qed.
+
+Local Lemma gmap_dep_lookup_GNode {A P} (ml : gmap_dep A P~0) mr mx i :
+  gmap_dep_lookup i (GNode ml mx mr) =
+    match i with
+    | 1 => snd <$> mx | i~0 => gmap_dep_lookup i ml | i~1 => gmap_dep_lookup i mr
+    end.
+Proof. by destruct ml, mx as [[]|], mr, i. Qed.
+
+Local Lemma gmap_dep_ne_lookup_not_None {A P} (t : gmap_dep_ne A P) :
+  ∃ i, P i ∧ gmap_dep_ne_lookup i t ≠ None.
+Proof.
+  induction t; repeat select (∃ _, _) (fun H => destruct H);
+    try first [by eexists 1|by eexists _~0|by eexists _~1].
+Qed.
+Local Lemma gmap_dep_eq_empty {A P} (mt : gmap_dep A P) :
+  (∀ i, P i → gmap_dep_lookup i mt = None) → mt = GEmpty.
+Proof.
+  intros Hlookup. destruct mt as [|t]; [done|].
+  destruct (gmap_dep_ne_lookup_not_None t); naive_solver.
+Qed.
+Local Lemma gmap_dep_eq {A P} (mt1 mt2 : gmap_dep A P) :
+  (∀ i, ProofIrrel (P i)) →
+  (∀ i, P i → gmap_dep_lookup i mt1 = gmap_dep_lookup i mt2) → mt1 = mt2.
+Proof.
+  revert mt2. induction mt1 as [|P ml1 mx1 mr1 _ IHl IHr] using gmap_dep_ind;
+    intros mt2 ? Hlookup;
+    destruct mt2 as [|? ml2 mx2 mr2 _ _ _] using gmap_dep_ind.
+  - done.
+  - symmetry. apply gmap_dep_eq_empty. naive_solver.
+  - apply gmap_dep_eq_empty. naive_solver.
+  - f_equal.
+    + apply (IHl _ _). intros i. generalize (Hlookup (i~0)).
+      by rewrite !gmap_dep_lookup_GNode.
+    + generalize (Hlookup 1). rewrite !gmap_dep_lookup_GNode.
+      destruct mx1 as [[]|], mx2 as [[]|]; intros; simplify_eq/=;
+        repeat f_equal; try  apply proof_irrel; naive_solver.
+    + apply (IHr _ _). intros i. generalize (Hlookup (i~1)).
+      by rewrite !gmap_dep_lookup_GNode.
+Qed.
+
+Local Lemma gmap_dep_ne_lookup_singleton {A P} i (p : P i) (x : A) :
+  gmap_dep_ne_lookup i (gmap_dep_ne_singleton i p x) = Some x.
+Proof. revert P p. induction i; by simpl. Qed.
+Local Lemma gmap_dep_ne_lookup_singleton_ne {A P} i j (p : P i) (x : A) :
+  i ≠ j → gmap_dep_ne_lookup j (gmap_dep_ne_singleton i p x) = None.
+Proof. revert P j p. induction i; intros ? [?|?|]; naive_solver. Qed.
+
+Local Lemma gmap_dep_partial_alter_GNode {A P} (f : option A → option A)
+    i (p : P i) (ml : gmap_dep A P~0) mx mr :
+  GNode_valid ml mx mr →
+  gmap_dep_partial_alter f i p (GNode ml mx mr) =
+    match i with
+    | 1 => λ p, GNode ml ((p,.) <$> f (snd <$> mx)) mr
+    | i~0 => λ p, GNode (gmap_dep_partial_alter f i p ml) mx mr
+    | i~1 => λ p, GNode ml mx (gmap_dep_partial_alter f i p mr)
+    end p.
+Proof. by destruct ml, mx as [[]|], mr. Qed.
+Local Lemma gmap_dep_lookup_partial_alter {A P} (f : option A → option A)
+    (mt : gmap_dep A P) i (p : P i) :
+  gmap_dep_lookup i (gmap_dep_partial_alter f i p mt) = f (gmap_dep_lookup i mt).
+Proof.
+  revert i p. induction mt using gmap_dep_ind.
+  { intros i p; simpl. destruct (f None); simpl; [|done].
+    by rewrite gmap_dep_ne_lookup_singleton. }
+  intros [] ?;
+    rewrite gmap_dep_partial_alter_GNode, !gmap_dep_lookup_GNode by done;
+    done || by destruct (f _).
+Qed.
+Local Lemma gmap_dep_lookup_partial_alter_ne {A P} (f : option A → option A)
+    (mt : gmap_dep A P) i (p : P i) j :
+  i ≠ j →
+  gmap_dep_lookup j (gmap_dep_partial_alter f i p mt) = gmap_dep_lookup j mt.
+Proof.
+  revert i p j; induction mt using gmap_dep_ind.
+  { intros i p j ?; simpl. destruct (f None); simpl; [|done].
+    by rewrite gmap_dep_ne_lookup_singleton_ne. }
+  intros [] ? [] ?;
+    rewrite gmap_dep_partial_alter_GNode, !gmap_dep_lookup_GNode by done;
+    auto with lia.
+Qed.
+
+Local Lemma gmap_dep_lookup_fmap {A B P} (f : A → B) (mt : gmap_dep A P) i :
+  gmap_dep_lookup i (gmap_dep_fmap f mt) = f <$> gmap_dep_lookup i mt.
+Proof.
+  destruct mt as [|t]; simpl; [done|].
+  revert i. induction t; intros []; by simpl.
+Qed.
+
+Local Lemma gmap_dep_omap_GNode {A B P} (f : A → option B)
+    (ml : gmap_dep A P~0) mx mr :
+  GNode_valid ml mx mr →
+  gmap_dep_omap f (GNode ml mx mr) =
+    GNode (gmap_dep_omap f ml) ('(p,x) ← mx; (p,.) <$> f x) (gmap_dep_omap f mr).
+Proof. by destruct ml, mx as [[]|], mr. Qed.
+Local Lemma gmap_dep_lookup_omap {A B P} (f : A → option B) (mt : gmap_dep A P) i :
+  gmap_dep_lookup i (gmap_dep_omap f mt) = gmap_dep_lookup i mt ≫= f.
+Proof.
+  revert i. induction mt using gmap_dep_ind; [done|].
+  intros [];
+    rewrite gmap_dep_omap_GNode, !gmap_dep_lookup_GNode by done; [done..|].
+  destruct select (option _) as [[]|]; simpl; by try destruct (f _).
+Qed.
+
+Section gmap_merge.
+  Context {A B C} (f : option A → option B → option C).
+
+  Local Lemma gmap_dep_merge_GNode_GEmpty {P} (ml : gmap_dep A P~0) mx mr :
+    GNode_valid ml mx mr →
+    gmap_dep_merge f (GNode ml mx mr) GEmpty =
+      GNode (gmap_dep_omap (λ x, f (Some x) None) ml) (diag_None' f mx None)
+            (gmap_dep_omap (λ x, f (Some x) None) mr).
+  Proof. by destruct ml, mx as [[]|], mr. Qed.
+  Local Lemma gmap_dep_merge_GEmpty_GNode {P} (ml : gmap_dep B P~0) mx mr :
+    GNode_valid ml mx mr →
+    gmap_dep_merge f GEmpty (GNode ml mx mr) =
+      GNode (gmap_dep_omap (λ x, f None (Some x)) ml) (diag_None' f None mx)
+            (gmap_dep_omap (λ x, f None (Some x)) mr).
+  Proof. by destruct ml, mx as [[]|], mr. Qed.
+  Local Lemma gmap_dep_merge_GNode_GNode {P}
+      (ml1 : gmap_dep A P~0) ml2 mx1 mx2 mr1 mr2 :
+    GNode_valid ml1 mx1 mr1 → GNode_valid ml2 mx2 mr2 →
+    gmap_dep_merge f (GNode ml1 mx1 mr1) (GNode ml2 mx2 mr2) =
+      GNode (gmap_dep_merge f ml1 ml2) (diag_None' f mx1 mx2)
+            (gmap_dep_merge f mr1 mr2).
+  Proof. by destruct ml1, mx1 as [[]|], mr1, ml2, mx2 as [[]|], mr2. Qed.
+
+  Local Lemma gmap_dep_lookup_merge {P} (mt1 : gmap_dep A P) (mt2 : gmap_dep B P) i :
+    gmap_dep_lookup i (gmap_dep_merge f mt1 mt2) =
+      diag_None f (gmap_dep_lookup i mt1) (gmap_dep_lookup i mt2).
+  Proof.
+    revert mt2 i; induction mt1 using gmap_dep_ind; intros mt2 i.
+    { induction mt2 using gmap_dep_ind; [done|].
+      rewrite gmap_dep_merge_GEmpty_GNode, gmap_dep_lookup_GNode by done.
+      destruct i as [i|i|];
+        rewrite ?gmap_dep_lookup_omap, gmap_dep_lookup_GNode; simpl;
+        [by destruct (gmap_dep_lookup i _)..|].
+      destruct select (option _) as [[]|]; simpl; by try destruct (f _). }
+    destruct mt2 using gmap_dep_ind.
+    { rewrite gmap_dep_merge_GNode_GEmpty, gmap_dep_lookup_GNode by done.
+      destruct i as [i|i|];
+        rewrite ?gmap_dep_lookup_omap, gmap_dep_lookup_GNode; simpl;
+        [by destruct (gmap_dep_lookup i _)..|].
+      destruct select (option _) as [[]|]; simpl; by try destruct (f _). }
+    rewrite gmap_dep_merge_GNode_GNode by done.
+    destruct i; rewrite ?gmap_dep_lookup_GNode; [done..|].
+    repeat destruct select (option _) as [[]|]; simpl; by try destruct (f _).
+  Qed.
+End gmap_merge.
+
+Section gmap_fold.
+  Context {A B} (f : positive → A → B → B).
+
+  Local Lemma gmap_dep_fold_GNode {P} i y (ml : gmap_dep A P~0) mx mr :
+    GNode_valid ml mx mr →
+    gmap_dep_fold f i y (GNode ml mx mr) = gmap_dep_fold f i~1
+      (gmap_dep_fold f i~0
+        match mx with None => y | Some (_,x) => f (Pos.reverse i) x y end ml) mr.
+  Proof. by destruct ml, mx as [[]|], mr. Qed.
+
+  Local Lemma gmap_dep_fold_ind {P} (Q : B → gmap_dep A P → Prop) (b : B) j :
+    Q b GEmpty →
+    (∀ i p x mt r, gmap_dep_lookup i mt = None →
+      Q r mt →
+      Q (f (Pos.reverse_go i j) x r) (gmap_dep_partial_alter (λ _, Some x) i p mt)) →
+    ∀ mt, Q (gmap_dep_fold f j b mt) mt.
+  Proof.
+    intros Hemp Hinsert mt. revert Q b j Hemp Hinsert.
+    induction mt as [|P ml mx mr ? IHl IHr] using gmap_dep_ind;
+      intros Q b j Hemp Hinsert; [done|].
+    rewrite gmap_dep_fold_GNode by done.
+    apply (IHr (λ y mt, Q y (GNode ml mx mt))).
+    { apply (IHl (λ y mt, Q y (GNode mt mx GEmpty))).
+      { destruct mx as [[p x]|]; [|done].
+        replace (GNode GEmpty (Some (p,x)) GEmpty) with
+          (gmap_dep_partial_alter (λ _, Some x) 1 p GEmpty) by done.
+        by apply Hinsert. }
+      intros i p x mt r ??.
+      replace (GNode (gmap_dep_partial_alter (λ _, Some x) i p mt) mx GEmpty)
+        with (gmap_dep_partial_alter (λ _, Some x) (i~0) p (GNode mt mx GEmpty))
+        by (by destruct mt, mx as [[]|]).
+      apply Hinsert; by rewrite ?gmap_dep_lookup_GNode. }
+    intros i p x mt r ??.
+    replace (GNode ml mx (gmap_dep_partial_alter (λ _, Some x) i p mt))
+      with (gmap_dep_partial_alter (λ _, Some x) (i~1) p (GNode ml mx mt))
+      by (by destruct ml, mx as [[]|], mt).
+    apply Hinsert; by rewrite ?gmap_dep_lookup_GNode.
+  Qed.
+End gmap_fold.
+
+(** Instance of the finite map type class *)
 Global Instance gmap_finmap `{Countable K} : FinMap K (gmap K).
 Proof.
   split.
-  - unfold lookup; intros A [m1 Hm1] [m2 Hm2] Hm.
-    apply gmap_eq, map_eq; intros i; simpl in *.
-    apply bool_decide_unpack in Hm1; apply bool_decide_unpack in Hm2.
-    apply option_eq; intros x; split; intros Hi.
-    + pose proof (Hm1 i x Hi); simpl in *.
-      by destruct (decode i); simplify_eq/=; rewrite <-Hm.
-    + pose proof (Hm2 i x Hi); simpl in *.
-      by destruct (decode i); simplify_eq/=; rewrite Hm.
+  - intros A [mt1] [mt2] Hlookup. f_equal. apply (gmap_dep_eq _ _ _).
+    intros i [Hk]. destruct (decode i) as [k|]; simplify_eq/=. apply Hlookup.
   - done.
-  - intros A f [m Hm] i; apply (lookup_partial_alter f m).
-  - intros A f [m Hm] i j Hs; apply (lookup_partial_alter_ne f m).
-    by contradict Hs; apply (inj encode).
-  - intros A B f [m Hm] i; apply (lookup_fmap f m).
-  - intros A B f [m Hm] i; apply (lookup_omap f m).
-  - intros A B C f [m1 Hm1] [m2 Hm2] i; unfold merge, lookup; simpl.
-    by rewrite lookup_merge by done; destruct (m1 !! _), (m2 !! _).
-  - intros A B P f b Hemp Hinsert [m Hm]. unfold map_fold; simpl. revert Hm.
-    apply (map_fold_ind (λ r m, ∀ Hm : gmap_wf K m, P r (GMap m Hm))); clear m.
-    { intros Hm.
-      by replace (GMap ∅ Hm) with (∅ : gmap K A) by (by apply gmap_eq). }
-    intros i x m r ? IH Hm'.
-    assert (gmap_wf K m) as Hm.
-    { apply bool_decide_pack; intros j y ?. apply bool_decide_unpack in Hm'.
-      apply (Hm' j y). rewrite lookup_insert_ne; naive_solver. }
-    assert (∃ k : K, i = encode k) as [k ->].
-    { apply bool_decide_unpack in Hm'.
-      specialize (Hm' i x (lookup_insert _ _ _)). apply fmap_Some in Hm'.
-      naive_solver. }
-    replace (GMap (<[encode k:=x]> m) Hm')
-      with (<[k:=x]> (GMap m Hm) : gmap K A) by (by apply gmap_eq).
-    rewrite decode_encode. by apply Hinsert, IH.
+  - intros A f [mt] i. apply gmap_dep_lookup_partial_alter.
+  - intros A f [mt] i j ?. apply gmap_dep_lookup_partial_alter_ne. naive_solver.
+  - intros A b f [mt] i. apply gmap_dep_lookup_fmap.
+  - intros A B f [mt] i. apply gmap_dep_lookup_omap.
+  - intros A B C f [mt1] [mt2] i. apply gmap_dep_lookup_merge.
+  - intros A B P f b Hemp Hinsert [mt].
+    apply (gmap_dep_fold_ind _ (λ r mt, P r (GMap mt))); clear mt; [done|].
+    intros i [Hk] x mt r ??; simpl. destruct (fmap_Some_1 _ _ _ Hk) as (k&->&->).
+    assert (GMapKey Hk = gmap_key_encode k) as -> by (apply proof_irrel).
+    by apply (Hinsert _ _ (GMap mt)).
 Qed.
 
 Global Program Instance gmap_countable
@@ -145,6 +511,60 @@ Next Obligation.
   intros K ?? A ?? m; simpl. rewrite decode_encode; simpl.
   by rewrite list_to_map_to_list.
 Qed.
+
+(** Conversion to/from [Pmap] *)
+Local Definition gmap_dep_ne_to_pmap_ne {A} : ∀ {P}, gmap_dep_ne A P → Pmap_ne A :=
+  fix go {P} t :=
+    match t with
+    | GNode001 r => PNode001 (go r)
+    | GNode010 _ x => PNode010 x
+    | GNode011 _ x r => PNode011 x (go r)
+    | GNode100 l => PNode100 (go l)
+    | GNode101 l r => PNode101 (go l) (go r)
+    | GNode110 l _ x => PNode110 (go l) x
+    | GNode111 l _ x r => PNode111 (go l) x (go r)
+    end.
+Local Definition gmap_dep_to_pmap {A P} (mt : gmap_dep A P) : Pmap A :=
+  match mt with
+  | GEmpty => PEmpty
+  | GNodes t => PNodes (gmap_dep_ne_to_pmap_ne t)
+  end.
+Definition gmap_to_pmap {A} (m : gmap positive A) : Pmap A :=
+  let '(GMap mt) := m in gmap_dep_to_pmap mt.
+
+Local Lemma lookup_gmap_dep_ne_to_pmap_ne {A P} (t : gmap_dep_ne A P) i :
+  gmap_dep_ne_to_pmap_ne t !! i = gmap_dep_ne_lookup i t.
+Proof. revert i; induction t; intros []; by simpl. Qed.
+Lemma lookup_gmap_to_pmap {A} (m : gmap positive A) i :
+  gmap_to_pmap m !! i = m !! i.
+Proof. destruct m as [[|t]]; [done|]. apply lookup_gmap_dep_ne_to_pmap_ne. Qed.
+
+Local Definition pmap_ne_to_gmap_dep_ne {A} :
+    ∀ {P}, (∀ i, P i) → Pmap_ne A → gmap_dep_ne A P :=
+  fix go {P} (p : ∀ i, P i) t :=
+    match t with
+    | PNode001 r => GNode001 (go p~1 r)
+    | PNode010 x => GNode010 (p 1) x
+    | PNode011 x r => GNode011 (p 1) x (go p~1 r)
+    | PNode100 l => GNode100 (go p~0 l)
+    | PNode101 l r => GNode101 (go p~0 l) (go p~1 r)
+    | PNode110 l x => GNode110 (go p~0 l) (p 1) x
+    | PNode111 l x r => GNode111 (go p~0 l) (p 1) x (go p~1 r)
+    end%function.
+Local Definition pmap_to_gmap_dep {A P}
+    (p : ∀ i, P i) (mt : Pmap A) : gmap_dep A P :=
+  match mt with
+  | PEmpty => GEmpty
+  | PNodes t => GNodes (pmap_ne_to_gmap_dep_ne p t)
+  end.
+Definition pmap_to_gmap {A} (m : Pmap A) : gmap positive A :=
+  GMap $ pmap_to_gmap_dep gmap_key_encode m.
+
+Local Lemma lookup_pmap_ne_to_gmap_dep_ne {A P} (p : ∀ i, P i) (t : Pmap_ne A) i :
+  gmap_dep_ne_lookup i (pmap_ne_to_gmap_dep_ne p t) = t !! i.
+Proof. revert P i p; induction t; intros ? [] ?; by simpl. Qed.
+Lemma lookup_pmap_to_gmap {A} (m : Pmap A) i : pmap_to_gmap m !! i = m !! i.
+Proof. destruct m as [|t]; [done|]. apply lookup_pmap_ne_to_gmap_dep_ne. Qed.
 
 (** * Curry and uncurry *)
 Definition gmap_uncurry `{Countable K1, Countable K2} {A} :
@@ -159,10 +579,8 @@ Definition gmap_curry `{Countable K1, Countable K2} {A} :
 Section curry_uncurry.
   Context `{Countable K1, Countable K2} {A : Type}.
 
-  (* FIXME: the type annotations `option (gmap K2 A)` are silly. Maybe these are
-  a consequence of Coq bug #5735 *)
   Lemma lookup_gmap_uncurry (m : gmap K1 (gmap K2 A)) i j :
-    gmap_uncurry m !! (i,j) = (m !! i : option (gmap K2 A)) ≫= (.!! j).
+    gmap_uncurry m !! (i,j) = m !! i ≫= (.!! j).
   Proof.
     apply (map_fold_ind (λ mr m, mr !! (i,j) = m !! i ≫= (.!! j))).
     { by rewrite !lookup_empty. }
@@ -179,7 +597,7 @@ Section curry_uncurry.
   Qed.
 
   Lemma lookup_gmap_curry (m : gmap (K1 * K2) A) i j :
-    (gmap_curry m !! i : option (gmap K2 A)) ≫= (.!! j) = m !! (i, j).
+    gmap_curry m !! i ≫= (.!! j) = m !! (i, j).
   Proof.
     apply (map_fold_ind (λ mr m, mr !! i ≫= (.!! j) = m !! (i, j))).
     { by rewrite !lookup_empty. }
@@ -225,7 +643,7 @@ Section curry_uncurry.
     intros Hne. apply map_eq; intros i. destruct (m !! i) as [m2|] eqn:Hm.
     - destruct (gmap_curry (gmap_uncurry m) !! i) as [m2'|] eqn:Hcurry.
       + f_equal. apply map_eq. intros j.
-        trans ((gmap_curry (gmap_uncurry m) !! i : option (gmap _ _)) ≫= (.!! j)).
+        trans (gmap_curry (gmap_uncurry m) !! i ≫= (.!! j)).
         { by rewrite Hcurry. }
         by rewrite lookup_gmap_curry, lookup_gmap_uncurry, Hm.
       + rewrite lookup_gmap_curry_None in Hcurry.
@@ -258,7 +676,7 @@ Section gset.
   (** We put in an eta expansion to avoid [injection] from unfolding equalities
   like [dom (gset _) m1 = dom (gset _) m2]. *)
   Global Instance gset_dom {A} : Dom (gmap K A) (gset K) := λ m,
-    let '(GMap m Hm) := m in mapset_dom (GMap m Hm).
+    let '(GMap mt) := m in mapset_dom (GMap mt).
 
   Global Arguments gset_elem_of : simpl never.
   Global Arguments gset_empty : simpl never.
